fstar/MLS.TreeKEM.Types.fst
@@ -4,6 +4,8 @@ open Comparse
 open MLS.Crypto
 open MLS.Tree
 
+#set-options "--fuel 0 --ifuel 0"
+
 noeq type member_info (bytes:Type0) {|crypto_bytes bytes|} = {
   public_key: hpke_public_key bytes;
   version: nat;
@@ -15,6 +17,8 @@ noeq type path_secret_ciphertext (bytes:Type0) {|crypto_bytes bytes|} = {
   ciphertext: bytes;
 }
 
+type direction = | Left | Right
+
 noeq type key_package (bytes:Type0) {|crypto_bytes bytes|} = {
   public_key: hpke_public_key bytes;
   version: nat;
@@ -24,5 +28,5 @@ noeq type key_package (bytes:Type0) {|crypto_bytes bytes|} = {
   path_secret_ciphertext: list (path_secret_ciphertext bytes);
 }
 
-type treekem (bytes:Type0) {|crypto_bytes bytes|} (l:nat) = tree l (option (member_info bytes)) (option (key_package bytes))
-type pathkem (bytes:Type0) {|crypto_bytes bytes|} (l:nat) = path l (member_info bytes) (option (key_package bytes))
+type treekem (bytes:Type0) {|crypto_bytes bytes|} (l:nat) (i:tree_index l) = tree l i (option (member_info bytes)) (option (key_package bytes))
+type pathkem (bytes:Type0) {|crypto_bytes bytes|} (l:nat) (i:tree_index l) (li:leaf_index l i) = path l i li (member_info bytes) (option (key_package bytes))
