fstar/MLS.TreeKEM.fst
@@ -9,23 +9,17 @@ open MLS.Result
 
 #set-options "--fuel 1 --ifuel 1 --z3rlimit 50"
 
-val leaf_public_key: #bytes:Type0 -> {|crypto_bytes bytes|} -> #l:nat -> treekem bytes l -> leaf_index l -> option (hpke_public_key bytes)
-let rec leaf_public_key #bytes #cb #l t leaf_index =
-  match t with
-  | TLeaf None -> None
-  | TLeaf (Some mi) -> Some (mi.public_key)
-  | TNode _ left right ->
-    let (dir, new_leaf_index) = child_index l leaf_index in
-    if dir = Left then
-      leaf_public_key left new_leaf_index
-    else
-      leaf_public_key right new_leaf_index
+val leaf_public_key: #bytes:Type0 -> {|crypto_bytes bytes|} -> #l:nat -> #i:tree_index l -> treekem bytes l i -> leaf_index l i -> option (hpke_public_key bytes)
+let leaf_public_key #bytes #cb #l #i t leaf_index =
+  match leaf_at t leaf_index with
+  | None -> None
+  | Some mi -> Some (mi.public_key)
 
 //This is a special case of the original_* functions below
-val unmerged_leaves_resolution: #bytes:Type0 -> {|crypto_bytes bytes|} -> #l:nat -> treekem bytes l -> list nat -> list (hpke_public_key bytes)
-let unmerged_leaves_resolution #bytes #cb #l t indexes =
+val unmerged_leaves_resolution: #bytes:Type0 -> {|crypto_bytes bytes|} -> #l:nat -> #i:tree_index l -> treekem bytes l i -> list nat -> list (hpke_public_key bytes)
+let unmerged_leaves_resolution #bytes #cb #l #i t indexes =
   List.Tot.concatMap (fun (index:nat) ->
-    if index < pow2 l then
+    if leaf_index_inside l i index  then
       match leaf_public_key t index with
       | None -> []
       | Some res -> [res]
@@ -34,73 +28,75 @@ let unmerged_leaves_resolution #bytes #cb #l t indexes =
   ) indexes
 
 //This is a special case of the original_* functions below
-val tree_resolution: #bytes:Type0 -> {|crypto_bytes bytes|} -> #l:nat -> treekem bytes l -> list (hpke_public_key bytes)
-let rec tree_resolution #bytes #cb #l t =
+val tree_resolution: #bytes:Type0 -> {|crypto_bytes bytes|} -> #l:nat -> #i:tree_index l -> treekem bytes l i -> list (hpke_public_key bytes)
+let rec tree_resolution #bytes #cb #l #i t =
   match t with
   | TLeaf None -> []
   | TLeaf (Some mi) -> [mi.public_key]
   | TNode (Some kp) left right -> (kp.public_key)::(unmerged_leaves_resolution t kp.unmerged_leaves)
   | TNode None left right -> (tree_resolution left)@(tree_resolution right)
 
-val original_unmerged_leaves_resolution: #bytes:Type0 -> {|crypto_bytes bytes|} -> #l:nat -> list nat -> treekem bytes l -> list nat -> list (hpke_public_key bytes)
-let original_unmerged_leaves_resolution #bytes #cb #l forbidden_leaves t indexes =
-  List.Tot.concatMap (fun (index:nat) ->
-    if index < pow2 l && not (List.Tot.mem index forbidden_leaves) then
-      match leaf_public_key t index with
-      | None -> []
-      | Some res -> [res]
-    else
-      []
-  ) indexes
-
-val split_forbidden_leaves: l:pos -> list nat -> list nat & list nat
-let rec split_forbidden_leaves l forbidden_leaves =
-  match forbidden_leaves with
-  | [] -> ([], [])
+val find_index: #a:eqtype -> a -> l:list a -> option (nat_less (List.Tot.length l))
+let rec find_index #a x l =
+  match l with
+  | [] -> None
   | h::t ->
-    let (res_l, res_r) = split_forbidden_leaves l t in
-    if h < pow2 (l-1) then
-      (h::res_l, res_r)
-    else
-      (res_l, (h-(pow2 (l-1)))::res_r)
+    if x=h then (
+      Some 0
+    ) else (
+      match find_index x t with
+      | Some res -> Some (res+1)
+      | None -> None
+    )
 
-val original_tree_resolution: #bytes:Type0 -> {|crypto_bytes bytes|} -> #l:nat -> list nat -> treekem bytes l -> list (hpke_public_key bytes)
-let rec original_tree_resolution #bytes #cb #l forbidden_leaves t =
-  match t with
-  | TLeaf None -> []
-  | TLeaf (Some mi) -> if forbidden_leaves = [] then [mi.public_key] else []
-  | TNode (Some kp) left right -> (kp.public_key)::(original_unmerged_leaves_resolution forbidden_leaves t kp.unmerged_leaves)
-  | TNode None left right ->
-    let (left_forbidden_leaves, right_forbidden_leaves) = split_forbidden_leaves l forbidden_leaves in
-    (original_tree_resolution left_forbidden_leaves left)@(original_tree_resolution right_forbidden_leaves right)
-
-val original_resolution_index: #bytes:Type0 -> {|crypto_bytes bytes|} -> #l:nat -> forbidden_leaves:list nat -> t:treekem bytes l -> leaf_index l -> nat_less (List.Tot.length (original_tree_resolution forbidden_leaves t))
-let rec original_resolution_index #bytes #cb #l forbidden_leaves t leaf_index =
+val resolution_index: #bytes:Type0 -> {|crypto_bytes bytes|} -> #l:nat -> #i:tree_index l -> t:treekem bytes l i -> leaf_index l i -> nat_less (List.Tot.length (tree_resolution t))
+let rec resolution_index #bytes #cb #l t leaf_index =
   match t with
   | TLeaf (Some mi) -> (
-    assume (forbidden_leaves = []); //TODO: We should be able to prove it
     0
   )
   | TLeaf None -> admit() //TODO: There should be a precondition that prevent this case
   | TNode (Some kp) left right -> (
-    match find_index forbidden_leaves leaf_index kp.unmerged_leaves with
+    match find_index leaf_index kp.unmerged_leaves with
     | Some res ->
       //That is currently not provable because a node might contain an unmerged leaf which is actually blanked
-      assume (1+res < List.Tot.length (original_tree_resolution forbidden_leaves t));
+      assume (1+res < List.Tot.length (tree_resolution t));
       1+res
     | None -> 0
   )
   | TNode None left right ->
-    let (child_dir, child_leaf_index) = child_index l leaf_index in
-    let (child, _) = order_subtrees child_dir (left, right) in
-    let (left_forbidden_leaves, right_forbidden_leaves) = split_forbidden_leaves l forbidden_leaves in
-    let child_forbidden_leaves = if child_dir = Left then left_forbidden_leaves else right_forbidden_leaves in
-    let child_resolution_index = original_resolution_index child_forbidden_leaves child child_leaf_index in
-    List.Tot.Properties.append_length (original_tree_resolution left_forbidden_leaves left) (original_tree_resolution right_forbidden_leaves right);
-    if child_dir = Left then
+    let (child, _) = get_child_sibling t leaf_index in
+    let child_resolution_index = resolution_index child leaf_index in
+    List.Tot.Properties.append_length (tree_resolution left) (tree_resolution right);
+    if is_left_leaf leaf_index then
       child_resolution_index
     else
-      (List.Tot.length (original_tree_resolution left_forbidden_leaves left)) + child_resolution_index
+      (List.Tot.length (tree_resolution left)) + child_resolution_index
+
+val un_addP: #bytes:Type0 -> {|crypto_bytes bytes|} -> #l:nat -> #i:tree_index l -> treekem bytes l i -> (nat -> bool) -> treekem bytes l i
+let rec un_addP #bytes #cb #l #i t pre =
+  match t with
+  | TLeaf _ -> if pre i then t else TLeaf None
+  | TNode okp left right -> (
+    let new_okp =
+      match okp with
+      | None -> None
+      | Some kp -> Some ({ kp with unmerged_leaves = List.Tot.filter pre kp.unmerged_leaves })
+    in
+    TNode new_okp (un_addP left pre) (un_addP right pre)
+  )
+
+val forbidden_pre: list nat -> nat -> bool
+let forbidden_pre l i =
+  not (List.Tot.mem i l)
+
+val original_tree_resolution: #bytes:Type0 -> {|crypto_bytes bytes|} -> #l:nat -> #i:tree_index l -> list nat -> treekem bytes l i -> list (hpke_public_key bytes)
+let original_tree_resolution #bytes #cb #l #i forbidden_leaves t =
+  tree_resolution (un_addP t (forbidden_pre forbidden_leaves))
+
+val original_resolution_index: #bytes:Type0 -> {|crypto_bytes bytes|} -> #l:nat -> #i:tree_index l -> forbidden_leaves:list nat -> t:treekem bytes l i -> leaf_index l i -> nat_less (List.Tot.length (original_tree_resolution forbidden_leaves t))
+let original_resolution_index #bytes #cb #l forbidden_leaves t leaf_index =
+  resolution_index (un_addP t (forbidden_pre forbidden_leaves)) leaf_index
 
 val hpke_multirecipient_encrypt_entropy_lengths: #bytes:Type0 -> {|crypto_bytes bytes|} -> list (hpke_public_key bytes) -> list nat
 let rec hpke_multirecipient_encrypt_entropy_lengths #bytes #cb pks =
@@ -159,25 +155,24 @@ let node_decap #bytes #cb child_secret i dir kp =
     hpke_decrypt ciphertext.kem_output child_sk (kp.last_group_context) empty ciphertext.ciphertext
   )
 
-val update_path_entropy_lengths: #bytes:Type0 -> {|crypto_bytes bytes|} -> #l:nat -> treekem bytes l -> leaf_index l -> list nat
-let rec update_path_entropy_lengths #bytes #cb #l t leaf_index =
+val update_path_entropy_lengths: #bytes:Type0 -> {|crypto_bytes bytes|} -> #l:nat -> #i:tree_index l -> treekem bytes l i -> leaf_index l i -> list nat
+let rec update_path_entropy_lengths #bytes #cb #l #i t leaf_index =
   match t with
   | TLeaf _ -> []
   | TNode _ left right ->
-    let (dir, new_leaf_index) = child_index l leaf_index in
-    let (child, sibling) = order_subtrees dir (left, right) in
+    let (child, sibling) = get_child_sibling t leaf_index in
     if tree_resolution sibling = [] then
-      update_path_entropy_lengths child new_leaf_index
+      update_path_entropy_lengths child leaf_index
     else
-      hpke_multirecipient_encrypt_entropy_lengths (tree_resolution sibling) @ update_path_entropy_lengths child new_leaf_index
+      hpke_multirecipient_encrypt_entropy_lengths (tree_resolution sibling) @ update_path_entropy_lengths child leaf_index
 
-val update_path: #bytes:Type0 -> {|crypto_bytes bytes|} -> #l:nat -> t:treekem bytes l -> leaf_index:leaf_index l -> leaf_secret:bytes -> ad:bytes -> randomness bytes (update_path_entropy_lengths t leaf_index) -> Pure (result (pathkem bytes l & bytes))
+val update_path: #bytes:Type0 -> {|crypto_bytes bytes|} -> #l:nat -> #i:tree_index l -> t:treekem bytes l i -> leaf_index:leaf_index l i -> leaf_secret:bytes -> ad:bytes -> randomness bytes (update_path_entropy_lengths t leaf_index) -> Pure (result (pathkem bytes l i leaf_index & bytes))
   (requires length leaf_secret >= hpke_private_key_length #bytes)
   (ensures fun res -> match res with
     | Success (_, node_secret) -> length leaf_secret >= hpke_private_key_length #bytes
     | _ -> True
   )
-let rec update_path #bytes #cb #l t leaf_index leaf_secret ad rand =
+let rec update_path #bytes #cb #l #i t leaf_index leaf_secret ad rand =
   match t with
   | TLeaf None -> admit() //TODO: in the previous code, it fails in this case
   | TLeaf (Some mi) ->
@@ -190,24 +185,24 @@ let rec update_path #bytes #cb #l t leaf_index leaf_secret ad rand =
       | None -> 0
       | Some kp -> kp.version+1
     in
-    let (dir, next_leaf_index) = child_index l leaf_index in
-    let (child, sibling) = order_subtrees dir (left, right) in
+    let (child, sibling) = get_child_sibling t leaf_index in
     if tree_resolution sibling = [] then (
-      let next_rand: randomness bytes (update_path_entropy_lengths #_ #_ #(l-1) child next_leaf_index) = rand in
-      recursive_call <-- update_path child next_leaf_index leaf_secret ad next_rand;
+      let next_rand: randomness bytes (update_path_entropy_lengths #_ #_ #(l-1) child leaf_index) = rand in
+      recursive_call <-- update_path child leaf_index leaf_secret ad next_rand;
       let (child_path, child_path_secret) = recursive_call in
       return (PNode None child_path, child_path_secret)
     ) else (
       let (rand_cur, rand_next) = split_randomness rand in
-      recursive_call <-- update_path child next_leaf_index leaf_secret ad rand_next;
+      recursive_call <-- update_path child leaf_index leaf_secret ad rand_next;
       let (child_path, child_path_secret) = recursive_call in
+      let dir = (if is_left_leaf leaf_index then Left else Right) in
       node_encap_call <-- node_encap version child_path_secret ad dir (tree_resolution sibling) rand_cur;
       let (node_kp, node_path_secret) = node_encap_call in
       return (PNode (Some node_kp) child_path, node_path_secret)
     )
 
-val root_secret: #bytes:Type0 -> {|crypto_bytes bytes|} -> #l:nat -> t:treekem bytes l -> leaf_index l -> leaf_secret:bytes -> result (bytes)
-let rec root_secret #bytes #cb #l t leaf_index leaf_secret =
+val root_secret: #bytes:Type0 -> {|crypto_bytes bytes|} -> #l:nat -> #i:tree_index l -> t:treekem bytes l i -> leaf_index l i -> leaf_secret:bytes -> result (bytes)
+let rec root_secret #bytes #cb #l #i t leaf_index leaf_secret =
   match t with
   | TLeaf None -> internal_failure "root_secret: leaf_index corresponds to an empty leaf"
   | TLeaf (Some _) -> return leaf_secret
@@ -215,41 +210,36 @@ let rec root_secret #bytes #cb #l t leaf_index leaf_secret =
     if List.Tot.mem leaf_index kp.unmerged_leaves then (
       return leaf_secret
     ) else (
-      let (dir, next_leaf_index) = child_index l leaf_index in
-      let (child, sibling) = order_subtrees dir (left, right) in
-      child_path_secret <-- root_secret child next_leaf_index leaf_secret;
+      let dir = if is_left_leaf leaf_index then Left else Right in
+      let (child, _) = get_child_sibling t leaf_index in
+      child_path_secret <-- root_secret child leaf_index leaf_secret;
       //The condition is here becaus the `i` argument has not sense when dir = kp.path_secret_from.
       //Maybe we should refactor `node_decap`?
-      let (left_forbidden_leaves, right_forbidden_leaves) = split_forbidden_leaves l kp.unmerged_leaves in
-      let child_forbidden_leaves = if dir = Left then left_forbidden_leaves else right_forbidden_leaves in
-      let i = if dir = kp.path_secret_from then 0 else original_resolution_index child_forbidden_leaves child next_leaf_index in
-      assume (dir <> kp.path_secret_from ==> List.Tot.length (original_tree_resolution child_forbidden_leaves child) == List.Tot.length kp.path_secret_ciphertext);
+      let i = if dir = kp.path_secret_from then 0 else original_resolution_index kp.unmerged_leaves child leaf_index in
+      assume (dir <> kp.path_secret_from ==> List.Tot.length (original_tree_resolution kp.unmerged_leaves child) == List.Tot.length kp.path_secret_ciphertext);
       node_decap child_path_secret i dir kp
     )
   end
   | TNode None left right -> begin
-    let (dir, next_leaf_index) = child_index l leaf_index in
-    let (child, sibling) = order_subtrees dir (left, right) in
-    root_secret child next_leaf_index leaf_secret
+    let (child, _) = get_child_sibling t leaf_index in
+    root_secret child leaf_index leaf_secret
   end
 
-val find_least_common_ancestor: #bytes:Type0 -> {|crypto_bytes bytes|} -> #l:nat -> treekem bytes l -> my_ind:leaf_index l -> other_ind:leaf_index l{my_ind <> other_ind} -> (res_l:nat & treekem bytes res_l & leaf_index res_l)
-let rec find_least_common_ancestor #bytes #cb #l t my_ind other_ind =
+val find_least_common_ancestor: #bytes:Type0 -> {|crypto_bytes bytes|} -> #l:nat -> #i:tree_index l -> treekem bytes l i -> my_ind:leaf_index l i -> other_ind:leaf_index l i{my_ind <> other_ind} -> (res_l:nat & res_i:tree_index res_l & treekem bytes res_l res_i & squash (leaf_index_inside res_l res_i my_ind))
+let rec find_least_common_ancestor #bytes #cb #l #i t my_ind other_ind =
   match t with
   | TNode _ left right ->
-      let (my_dir, next_my_ind) = child_index l my_ind in
-      let (other_dir, next_other_ind) = child_index l other_ind in
-      if my_dir = other_dir then (
-        let (child, sibling) = order_subtrees my_dir (left, right) in
-        find_least_common_ancestor child next_my_ind next_other_ind
+      if is_left_leaf my_ind = is_left_leaf other_ind then (
+        let (child, sibling) = get_child_sibling t my_ind in
+        find_least_common_ancestor child my_ind other_ind
       ) else (
-        (|l, t, my_ind|)
+        (|l, i, t, ()|)
       )
 
-val path_secret_at_least_common_ancestor: #bytes:Type0 -> {|crypto_bytes bytes|} -> #l:nat -> treekem bytes l -> my_ind:leaf_index l -> other_ind:leaf_index l{my_ind <> other_ind} -> leaf_secret:bytes -> result bytes
+val path_secret_at_least_common_ancestor: #bytes:Type0 -> {|crypto_bytes bytes|} -> #l:nat -> #i:tree_index l -> treekem bytes l i -> my_ind:leaf_index l i -> other_ind:leaf_index l i{my_ind <> other_ind} -> leaf_secret:bytes -> result bytes
 let path_secret_at_least_common_ancestor #bytes #cb #l t my_ind other_ind leaf_secret =
-  let (|_, lca, lca_my_ind|) = find_least_common_ancestor t my_ind other_ind in
-  root_secret lca lca_my_ind leaf_secret
+  let (|_, _, lca, _|) = find_least_common_ancestor t my_ind other_ind in
+  root_secret lca my_ind leaf_secret
 
 val empty_path_secret_ciphertext: #bytes:Type0 -> {|crypto_bytes bytes|} -> path_secret_ciphertext bytes
 let empty_path_secret_ciphertext #bytes #cb = {
@@ -257,14 +247,14 @@ let empty_path_secret_ciphertext #bytes #cb = {
     ciphertext = empty;
   }
 
-val mk_init_path_aux: #bytes:Type0 -> {|crypto_bytes bytes|} -> #l:nat -> treekem bytes l -> update_index:leaf_index l -> result (pathkem bytes l)
+val mk_init_path_aux: #bytes:Type0 -> {|crypto_bytes bytes|} -> #l:nat -> #i:tree_index l -> treekem bytes l i -> update_index:leaf_index l i -> result (pathkem bytes l i update_index)
 let rec mk_init_path_aux #bytes #cb #l t update_index =
   match t with
   | TLeaf None -> error "mk_init_path_aux: update leaf cannot be blanked"
   | TLeaf (Some mi) -> return (PLeaf mi)
   | TNode okp left right -> begin
-    let (update_dir, next_update_index) = child_index l update_index in
-    let (child, sibling) = order_subtrees update_dir (left, right) in
+    let update_dir = if is_left_leaf update_index then Left else Right in
+    let (child, _) = get_child_sibling t update_index in
     let new_okp =
       match okp with
       | Some kp -> Some ({ kp with
@@ -272,18 +262,17 @@ let rec mk_init_path_aux #bytes #cb #l t update_index =
         })
       | None -> None
     in
-    next <-- mk_init_path_aux child next_update_index;
+    next <-- mk_init_path_aux child update_index;
     return (PNode okp next)
   end
 
-val mk_init_path: #bytes:Type0 -> {|crypto_bytes bytes|} -> #l:nat -> treekem bytes l -> my_index:leaf_index l -> update_index:leaf_index l{my_index <> update_index} -> path_secret:bytes -> hpke_info:bytes -> result (pathkem bytes l)
+val mk_init_path: #bytes:Type0 -> {|crypto_bytes bytes|} -> #l:nat -> #i:tree_index l -> treekem bytes l i -> my_index:leaf_index l i -> update_index:leaf_index l i{my_index <> update_index} -> path_secret:bytes -> hpke_info:bytes -> result (pathkem bytes l i update_index)
 let rec mk_init_path #bytes #cb #l t my_index update_index path_secret hpke_info =
   match t with
   | TNode okp left right -> begin
-    let (my_dir, next_my_index) = child_index l my_index in
-    let (update_dir, next_update_index) = child_index l update_index in
-    let (child, sibling) = order_subtrees update_dir (left, right) in
-    if my_dir = update_dir then (
+    let update_dir = if is_left_leaf update_index then Left else Right in
+    let (child, sibling) = get_child_sibling t update_index in
+    if is_left_leaf my_index = is_left_leaf update_index then (
       let new_okp =
         match okp with
         | Some kp -> Some ({ kp with
@@ -291,7 +280,7 @@ let rec mk_init_path #bytes #cb #l t my_index update_index path_secret hpke_info
         })
         | None -> None
       in
-      next <-- mk_init_path child next_my_index next_update_index path_secret hpke_info;
+      next <-- mk_init_path child my_index update_index path_secret hpke_info;
       return (PNode new_okp next)
     ) else (
       if not (Some? okp && (Some?.v okp).unmerged_leaves = []) then
@@ -299,7 +288,7 @@ let rec mk_init_path #bytes #cb #l t my_index update_index path_secret hpke_info
       else (
         let kp = Some?.v okp in
         let resol_size = List.Tot.length (original_tree_resolution [] sibling) in
-        let resol_index = original_resolution_index [] sibling next_my_index in
+        let resol_index = original_resolution_index [] sibling my_index in
         let fake_randomness = mk_zero_vector (hpke_private_key_length #bytes) in
         my_pk <-- from_option "leaf at my_index is empty!" (leaf_public_key t my_index);
         my_path_secret_ciphertext <-- hpke_encrypt my_pk hpke_info empty path_secret fake_randomness;
@@ -309,7 +298,7 @@ let rec mk_init_path #bytes #cb #l t my_index update_index path_secret hpke_info
           //TODO: put the {kem_output = ...; ...} in a separate function
           path_secret_ciphertext = Seq.seq_to_list (Seq.upd (Seq.create resol_size (empty_path_secret_ciphertext)) resol_index ({kem_output=fst my_path_secret_ciphertext; ciphertext = snd my_path_secret_ciphertext}));
         } in
-        next <-- mk_init_path_aux child next_update_index;
+        next <-- mk_init_path_aux child update_index;
         return (PNode (Some new_kp) next)
       )
     )
