fstar/MLS.TreeSync.ParentHash.fst
@@ -28,11 +28,11 @@ let get_encryption_key_from_content #bytes #bl content =
     (parse (treekem_content_nt bytes) content);
   return content.encryption_key
 
-val un_add: #bytes:Type0 -> {|bytes_like bytes|} -> #l:nat -> treesync bytes l -> list nat -> nat -> treesync bytes l
-let rec un_add #bytes #bl #l t leaves nb_left_leaves =
+val un_add: #bytes:Type0 -> {|bytes_like bytes|} -> #l:nat -> #i:tree_index l -> treesync bytes l i -> list nat -> treesync bytes l i
+let rec un_add #bytes #bl #l #i t leaves =
   match t with
   | TLeaf olp -> (
-    if List.Tot.mem nb_left_leaves leaves then
+    if List.Tot.mem i leaves then
       TLeaf None
     else
       TLeaf olp
@@ -46,14 +46,14 @@ let rec un_add #bytes #bl #l t leaves nb_left_leaves =
         Some ({ np with unmerged_leaves = new_unmerged_leaves } <: node_package_t bytes)
       )
     in
-    let new_left = un_add left leaves nb_left_leaves in
-    let new_right = un_add right leaves (nb_left_leaves + pow2 (l-1)) in
+    let new_left = un_add left leaves in
+    let new_right = un_add right leaves in
     TNode new_onp new_left new_right
 
-val compute_parent_hash_from_sibling: #bytes:Type0 -> {|crypto_bytes bytes|} -> #ls:nat -> node_package_t bytes -> nat -> treesync bytes ls -> result (lbytes bytes (hash_length #bytes))
-let compute_parent_hash_from_sibling #bytes #cb #ls root_np nb_left_leaves_sibling sibling =
+val compute_parent_hash: #bytes:Type0 -> {|crypto_bytes bytes|} -> #l:nat -> #i:tree_index l -> node_package_t bytes -> treesync bytes l i -> result (lbytes bytes (hash_length #bytes))
+let compute_parent_hash #bytes #cb #l #i root_np sibling =
   encryption_key <-- get_encryption_key_from_content root_np.content.content;
-  original_sibling_tree_hash <-- tree_hash (un_add sibling root_np.unmerged_leaves nb_left_leaves_sibling);
+  original_sibling_tree_hash <-- tree_hash (un_add sibling root_np.unmerged_leaves);
   if not (length root_np.parent_hash < pow2 30) then
     internal_failure "compute_parent_hash_from_sibling: parent_hash too long"
   else (
@@ -64,16 +64,3 @@ let compute_parent_hash_from_sibling #bytes #cb #ls root_np nb_left_leaves_sibli
     }))
   )
 
-val compute_parent_hash_from_dir: #bytes:Type0 -> {|crypto_bytes bytes|} -> #l:nat -> nat -> treesync bytes l -> direction -> result (lbytes bytes (hash_length #bytes))
-let compute_parent_hash_from_dir #bytes #cb #l nb_left_leaves root dir =
-  match root with
-  | TNode (Some root_np) left right ->
-    let (_, sibling) = order_subtrees dir (left, right) in
-    let nb_left_leaves_sibling =
-      if dir = Left then
-        nb_left_leaves + (pow2 (l-1))
-      else
-        nb_left_leaves
-    in
-    compute_parent_hash_from_sibling root_np nb_left_leaves_sibling sibling
-  | _ -> internal_failure "compute_parent_hash_from_dir: `root` must be a non-blank internal node"
