fstar/MLS.TreeSync.Types.fst
@@ -4,9 +4,9 @@ open Comparse.Bytes
 open MLS.NetworkTypes
 open MLS.Tree
 
-(** Identity and Credentials *)
-type principal_t = string
+#set-options "--fuel 1 --ifuel 1"
 
+(** Identity and Credentials *)
 type credential_t (bytes:Type0) {|bytes_like bytes|} = {
   version: nat; //For security proofs, should be erasable
   identity: bytes;
@@ -45,30 +45,28 @@ type node_package_t (bytes:Type0) {|bytes_like bytes|} = {
 }
 
 (** Tree and Paths definitions *)
-type level_n = nat
+type treesync (bytes:Type0) {|bytes_like bytes|} (l:nat) (i:tree_index l) = tree l i (option (leaf_package_t bytes)) (option (node_package_t bytes))
+type pathsync (bytes:Type0) {|bytes_like bytes|} (l:nat) (i:tree_index l) (li:leaf_index l i) = path l i li (option (leaf_package_t bytes)) (option (node_package_t bytes))
 
-type treesync (bytes:Type0) {|bytes_like bytes|} (l:level_n) = tree l (option (leaf_package_t bytes)) (option (node_package_t bytes))
-type pathsync (bytes:Type0) {|bytes_like bytes|} (l:level_n) = path l (option (leaf_package_t bytes)) (option (node_package_t bytes))
-
-type external_pathsync (bytes:Type0) {|bytes_like bytes|} (l:level_n) = path l (leaf_package_t bytes) (option (external_content bytes))
+type external_pathsync (bytes:Type0) {|bytes_like bytes|} (l:nat) (i:tree_index l) (li:leaf_index l i) = path l i li (leaf_package_t bytes) (option (external_content bytes))
 
 type operation_t (bytes:Type0) {|bytes_like bytes|} =
   | Op_Add: lp:leaf_package_t bytes -> operation_t bytes
   | Op_Update: lp:leaf_package_t bytes -> operation_t bytes
   | Op_Remove: ind:nat -> operation_t bytes
-  | Op_UpdatePath: l:level_n -> external_pathsync bytes l -> operation_t bytes
+  | Op_UpdatePath: l:nat -> i:tree_index l -> li:leaf_index l i -> external_pathsync bytes l i li -> operation_t bytes
 
 (** TreeSync state and accessors *)
 type state_t (bytes:Type0) {|bytes_like bytes|} = {
   group_id: bytes;
-  levels: level_n;
-  tree: treesync bytes levels;
+  levels: nat;
+  tree: treesync bytes levels 0;
   version: nat;
   //initial_tree: treesync levels treesize;
   transcript: Seq.seq (operation_t bytes);
 }
 
-val mk_initial_state: #bytes:Type0 -> {|bytes_like bytes|} -> gid:bytes -> l:level_n -> treesync bytes l -> state_t bytes
+val mk_initial_state: #bytes:Type0 -> {|bytes_like bytes|} -> gid:bytes -> l:nat -> treesync bytes l 0 -> state_t bytes
 let mk_initial_state gid l t = {
   group_id = gid; levels = l;
   tree = t; version = 0;
