fstar/MLS.TreeSync.fst
@@ -5,73 +5,72 @@ open MLS.Utils
 open MLS.Tree
 open MLS.TreeSync.Types
 
+#set-options "--fuel 1 --ifuel 1"
+
 (*** Tree creation ***)
 
-val create_tree: #bytes:Type0 -> {|bytes_like bytes|} -> leaf_package_t bytes -> treesync bytes 0
+val create_tree: #bytes:Type0 -> {|bytes_like bytes|} -> leaf_package_t bytes -> treesync bytes 0 0
 let create_tree lp =
   TLeaf (Some lp)
 
 (*** Tree operations ***)
 
-val tree_add: #bytes:Type0 -> {|bytes_like bytes|} -> #l:nat -> treesync bytes l -> nat -> i:leaf_index l -> leaf_package_t bytes -> treesync bytes l
-let rec tree_add #bytes #bl #l t original_i i lp =
+val tree_add: #bytes:Type0 -> {|bytes_like bytes|} -> #l:nat -> #i:tree_index l -> treesync bytes l i -> li:leaf_index l i -> leaf_package_t bytes -> treesync bytes l i
+let rec tree_add #bytes #bl #l #i t li lp =
   match t with
   | TLeaf _ -> TLeaf (Some lp)
   | TNode opt_content left right -> (
-    let (dir, new_i) = child_index l i in
     let new_opt_content =
       match opt_content with
       | None -> None
       | Some content -> Some ({
-        content with unmerged_leaves = insert_sorted original_i content.unmerged_leaves
+        content with unmerged_leaves = insert_sorted li content.unmerged_leaves
       })
     in
-    if dir = Left
-    then TNode new_opt_content (tree_add left original_i new_i lp) right
-    else TNode new_opt_content left (tree_add right original_i new_i lp)
+    if is_left_leaf li
+    then TNode new_opt_content (tree_add left li lp) right
+    else TNode new_opt_content left (tree_add right li lp)
    )
 
-val tree_blank_path: #bytes:Type0 -> {|bytes_like bytes|} -> #l:nat -> treesync bytes l -> i:leaf_index l -> option (leaf_package_t bytes) -> treesync bytes l
-let rec tree_blank_path #bytes #bl #l t i opt_lp =
+val tree_blank_path: #bytes:Type0 -> {|bytes_like bytes|} -> #l:nat -> #i:tree_index l -> treesync bytes l i -> leaf_index l i -> option (leaf_package_t bytes) -> treesync bytes l i
+let rec tree_blank_path #bytes #bl #l #i t li opt_lp =
   match t with
   | TLeaf _ -> TLeaf opt_lp
   | TNode opt_node_content left right -> (
-    let (dir, new_i) = child_index l i in
-    if dir = Left
-    then TNode None (tree_blank_path left new_i opt_lp) right
-    else TNode None left (tree_blank_path right new_i opt_lp)
+    if is_left_leaf li
+    then TNode None (tree_blank_path left li opt_lp) right
+    else TNode None left (tree_blank_path right li opt_lp)
   )
 
-val tree_update: #bytes:Type0 -> {|bytes_like bytes|} -> #l:nat -> treesync bytes l -> i:leaf_index l -> leaf_package_t bytes -> treesync bytes l
-let tree_update #bytes #bl #l t i lp =
-  tree_blank_path t i (Some lp)
+val tree_update: #bytes:Type0 -> {|bytes_like bytes|} -> #l:nat -> #i:tree_index l -> treesync bytes l i -> leaf_index l i -> leaf_package_t bytes -> treesync bytes l i
+let tree_update #bytes #bl #l #i t li lp =
+  tree_blank_path t li (Some lp)
 
-val tree_remove: #bytes:Type0 -> {|bytes_like bytes|} -> #l:nat -> treesync bytes l -> i:leaf_index l -> treesync bytes l
-let tree_remove #bytes #bl #l t i =
-  tree_blank_path t i None
+val tree_remove: #bytes:Type0 -> {|bytes_like bytes|} -> #l:nat -> #i:tree_index l -> treesync bytes l i -> leaf_index l i -> treesync bytes l i
+let tree_remove #bytes #bl #l #i t li =
+  tree_blank_path t li None
 
-val apply_path: #bytes:Type0 -> {|bytes_like bytes|} -> #l:nat -> treesync bytes l -> pathsync bytes l -> leaf_index l -> treesync bytes l
-let rec apply_path #bytes #bl #l t p i =
+val apply_path: #bytes:Type0 -> {|bytes_like bytes|} -> #l:nat -> #i:tree_index l -> #li:leaf_index l i -> treesync bytes l i -> pathsync bytes l i li -> treesync bytes l i
+let rec apply_path #bytes #bl #l #i #li t p =
   match t,p with
   | TLeaf _, PLeaf m' -> TLeaf m'
   | TNode _ left right, PNode onp next ->
-     let (dir,new_i) = child_index l i in
-     if dir = Left
-     then TNode onp (apply_path left next new_i) right
-     else TNode onp left (apply_path right next new_i)
+     if is_left_leaf li
+     then TNode onp (apply_path left next) right
+     else TNode onp left (apply_path right next)
 
 
 (*** Tree extension / truncation ***)
 
-val is_tree_empty: #bytes:Type0 -> {|bytes_like bytes|} -> #l:nat -> treesync bytes l -> bool
-let rec is_tree_empty #bytes #bl #l t =
+val is_tree_empty: #bytes:Type0 -> {|bytes_like bytes|} -> #l:nat -> #i:tree_index l -> treesync bytes l i -> bool
+let rec is_tree_empty #bytes #bl #l #i t =
   match t with
   | TNode _ left right ->
     is_tree_empty left && is_tree_empty right
   | TLeaf (Some _) -> false
   | TLeaf None -> true
 
-val canonicalize_tree: #bytes:Type0 -> {|bytes_like bytes|} -> #l:nat -> treesync bytes l -> (l_res:nat{l_res <= l} & treesync bytes l_res)
+val canonicalize_tree: #bytes:Type0 -> {|bytes_like bytes|} -> #l:nat -> treesync bytes l 0 -> (l_res:nat{l_res <= l} & treesync bytes l_res 0)
 let canonicalize_tree #bytes #bl #l t0 =
   match t0 with
   | TLeaf _ -> (|_, t0|)
@@ -81,26 +80,26 @@ let canonicalize_tree #bytes #bl #l t0 =
 
 // Helper functions to add leaf / extend the tree
 
-val find_empty_leaf: #bytes:Type0 -> {|bytes_like bytes|} -> #l:nat -> treesync bytes l -> option (leaf_index l)
-let rec find_empty_leaf #bytes #bl #l t =
+val find_empty_leaf: #bytes:Type0 -> {|bytes_like bytes|} -> #l:nat -> #i:tree_index l -> treesync bytes l i -> option (leaf_index l i)
+let rec find_empty_leaf #bytes #bl #l #i t =
   match t with
+  | TLeaf (Some _) -> None
+  | TLeaf None -> Some i
   | TNode _ left right -> (
     match find_empty_leaf left, find_empty_leaf right with
     | Some x, _ -> Some x
-    | None, Some x -> Some ((pow2 (l-1)) + x)
+    | None, Some x -> Some x
     | None, None -> None
   )
-  | TLeaf (Some _) -> None
-  | TLeaf None -> Some 0
 
-val mk_blank_tree: #bytes:Type0 -> {|bytes_like bytes|} -> l:nat -> Pure (treesync bytes l) (requires True) (ensures fun res -> Some? (find_empty_leaf res))
-let rec mk_blank_tree #bytes #bl l =
+val mk_blank_tree: #bytes:Type0 -> {|bytes_like bytes|} -> l:nat -> i:tree_index l -> Pure (treesync bytes l i) (requires True) (ensures fun res -> Some? (find_empty_leaf res))
+let rec mk_blank_tree #bytes #bl l i =
   if l = 0 then TLeaf None
-  else TNode None (mk_blank_tree (l-1)) (mk_blank_tree (l-1))
+  else TNode None (mk_blank_tree (l-1) _) (mk_blank_tree (l-1) _)
 
-val add_one_level: #bytes:Type0 -> {|bytes_like bytes|} -> #l:nat -> treesync bytes l -> Pure (treesync bytes (l+1)) (requires True) (fun res -> Some? (find_empty_leaf res))
+val add_one_level: #bytes:Type0 -> {|bytes_like bytes|} -> #l:nat -> treesync bytes l 0 -> Pure (treesync bytes (l+1) 0) (requires True) (fun res -> Some? (find_empty_leaf res))
 let add_one_level #bytes #bl #l t =
-  TNode None t (mk_blank_tree l)
+  TNode None t (mk_blank_tree l _)
 
 (*** Higher-level API ***)
 
@@ -113,7 +112,7 @@ val create: #bytes:Type0 -> {|bytes_like bytes|} -> gid:bytes -> leaf_package_t 
 let create #bytes #bl gid lp =
   mk_initial_state gid 0 (create_tree lp)
 
-val state_update_tree: #bytes:Type0 -> {|bytes_like bytes|} -> #l:level_n -> state_t bytes -> treesync bytes l -> state_t bytes
+val state_update_tree: #bytes:Type0 -> {|bytes_like bytes|} -> #l:nat -> state_t bytes -> treesync bytes l 0 -> state_t bytes
 let state_update_tree #bytes #bl #l st new_tree =
   ({ st with
     levels = l;
@@ -136,11 +135,11 @@ let add #bytes #bl st kp =
   lp <-- get_leaf_package_from_key_package kp;
   match find_empty_leaf st.tree with
   | Some i ->
-    return (state_update_tree st (tree_add st.tree i i lp), (i <: nat))
+    return (state_update_tree st (tree_add st.tree i lp), (i <: nat))
   | None ->
     let augmented_tree = add_one_level st.tree in
     let i = Some?.v (find_empty_leaf augmented_tree) in
-    return (state_update_tree st (tree_add augmented_tree i i lp), i)
+    return (state_update_tree st (tree_add augmented_tree i lp), i)
 
 val update: #bytes:Type0 -> {|bytes_like bytes|} -> st:state_t bytes -> leaf_package_t bytes -> index_t st -> state_t bytes
 let update #bytes #bl st lp i =
